arithmetic/coq/Verif_number_add_inner.v
@@ -3,3 +3,9 @@ Require Import VST.floyd.library.
 Require Import Didactica.arithmetic.
 Require Import Didactica.number.
 
+Lemma body_number_add_inner: semax_body Vprog Gprog f_number_add_inner number_add_inner_spec.
+Proof.
+  start_function.
+  forward. forward. unfold make_number. forward_call.
+  forward. forward.
+Admitted.
